\documentclass[11pt]{article}

\setlength{\marginparwidth}{1.2in}
\let\oldmarginpar\marginpar
\renewcommand\marginpar[1]{\-\oldmarginpar[\raggedleft\footnotesize #1]%
{\raggedright\footnotesize #1}}

\frenchspacing % no extra space at the end of a sentence

\setlength{\parindent}{0in}
\setlength{\parskip}{.1in}

\raggedbottom

%\pagestyle{empty}

% 	PACKAGES
% \usepackage[small,bf]{caption}
% \let\bcode\textbgreek
% \usepackage[bgreek,english]{babel}
% \usepackage{setspace}
\usepackage{amsfonts}
\usepackage{amssymb}
\usepackage{amsmath}
% \usepackage{german}
% \usepackage{hebtex}
% \usepackage{graphicx}
% \usepackage[german]{babel}
% \usepackage{endnotes}
% \let\footnote=\endnote
% \usepackage{rotating}
% \usepackage{enumerate}

\newcommand{\kapt}[1]{\textbf{{\thechap}. #1}\addtocounter{chap}{1}}

\newcommand{\tbd}[1]{}
\newcommand{\qnull}[1]{`#1'}
\newcommand{\qeins}[1]{``#1''}
\newcommand{\qzwei}[1]{`#1'}

\newif\ifNumericalOrYear
\NumericalOrYeartrue
% \NumericalOrYearfalse
\ifNumericalOrYear
\usepackage[numbers,colon]{natbib}
\else
\usepackage[round,colon]{natbib}
\fi
\newif\ifPageP
\PagePtrue
% \PagePfalse
\ifPageP
\newcommand{\PageP}{p.~}
\else
\newcommand{\PageP}{}
\fi

\newcommand{\scite}[3]{\ifnum#1=1\ifNumericalOrYear\citep{#2}\else\citeyearpar{#2}\fi\else
\ifnum#1=2\ifNumericalOrYear\citep[#3]{#2}\else\citep[{\PageP}#3]{#2}\fi\else
\ifnum#1=3\ifNumericalOrYear(\citet[#3]{#2})\else\citep[{\PageP}#3]{#2}\fi\else
\ifnum#1=4\ifNumericalOrYear\citet{#2}\else\citet{#2}\fi\else
\ifnum#1=5\ifNumericalOrYear(\citet{#2})\else\citep{#2}\fi\else
\ifnum#1=6\ifNumericalOrYear(\citet[#3]{#2})\else\citep[{\PageP}#3]{#2}\fi\else
\ifnum#1=7\ifNumericalOrYear\citep{#2}\else\citealp{#2}\fi\else
\ifnum#1=8\ifNumericalOrYear\citep[#3]{#2}\else\citealp[{\PageP}#3]{#2}\fi\else
\textbf{[invalid scite code]}\fi\fi\fi\fi\fi\fi\fi\fi}

\newenvironment{quotex}{\begin{quote}\begin{footnotesize}}{\end{footnotesize}\end{quote}}
% \newenvironment{quotex}{\begin{quote}\begin{footnotesize}\begin{singlespace}}{\end{singlespace}\end{footnotesize}\end{quote}}

\begin{document}

\title{Probability Kinematics and Halpern's Full Employment Theory}

\author{Stefan Lukits}

\maketitle

\newcounter{chap}

\setcounter{chap}{1}

\kapt{Introduction}

Let $f$ be a probability distribution on a finite space
$x_{1},\ldots,x_{m}$ that fulfills the constraint
\begin{equation}
  \label{eq:constraint}
\sum_{i=1}^{m}r(x_{i})f(x_{i})=\alpha
\end{equation}

Because $f$ is a probability distribution it fulfills
\begin{equation}
  \label{eq:unity}
\sum_{i=1}^{m}f(x_{i})=1
\end{equation}

We want to maximize the entropy, given the constraints
({\ref{eq:constraint}}) and ({\ref{eq:unity}}),
\begin{equation}
  \label{eq:entropy}
-\sum_{i=1}^{m}f(x_{i})\ln(x_{i})
\end{equation}

We use Lagrange multipliers to define the functional
\begin{equation}
  \label{eq:functional}
J(f(x_{i}))=-\sum_{i=1}^{m}f(x_{i})\ln{}f(x_{i})+\lambda_{0}\sum_{i=1}^{m}f+\lambda_{1}\sum_{i=1}^{m}r(x_{1})f(x_{i})
\end{equation}
and differentiate it with respect to $x_{i}$
\begin{equation}
  \label{eq:funder}
\frac{\partial{}J}{\partial{}f(x_{i})}=-\ln(f(x_{i}))-1+\lambda_{0}+\lambda_{1}r(x_{i})
\end{equation}

Set ({\ref{eq:funder}}) to $0$ to find the necessary condition to
maximize ({\ref{eq:entropy}})
\begin{equation}
  \label{eq:coverthomas}
g(x_{i})=e^{\lambda_{0}-1+\lambda_{1}r(x_{1})}
\end{equation}

This is the Gibbs distribution. We still need to do two things: (a)
show that the entropy of $g$ is maximal, and (b) show how to find
$\lambda_{0}$ and $\lambda_{1}$. (a) is shown in Theorem 12.1.1 in
Cover and Thomas \scite{1}{coverthomas91}{} and there is no reason to
copy it here. I was not able to find (b) in the literature and will
show it here. A faint suggestion on how to do it is in Jaynes'
treatment of the Brandeis Dice Problem (see \scite{8}{jaynes89}{243}). 

Let
\begin{equation}
  \label{eq:l1}
\lambda_{1}=-\beta
\end{equation}
\begin{equation}
  \label{eq:zet}
Z(\beta)=\sum_{i=1}^{m}e^{-\beta{}r(x_{i})}
\end{equation}
\begin{equation}
  \label{eq:l0}
\lambda_{0}=1-Z(\beta)
\end{equation}

To find $\lambda_{0}$ and $\lambda_{1}$ we introduce the constraint
\begin{equation}
  \label{eq:logcon}
-\frac{\partial}{\partial{}\beta}\ln(Z(\beta))=\alpha
\end{equation}

To see how this constraint gives us $\lambda_{0}$ and $\lambda_{1}$
Jaynes' solution of the Brandeis Dice Problem is a helpful example. We
are, however, interested in a general proof that this choice of
$\lambda_{0}$ and $\lambda_{1}$ gives us the probability distribution
maximizing the entropy. That $g$ so defined maximizes the entropy is
shown in (a). We need to make sure, however, that with this choice of
$\lambda_{0}$ and $\lambda_{1}$ the constraints
({\ref{eq:constraint}}) and ({\ref{eq:unity}}) are also fulfilled.

First, we show
% \begin{align}
% &\mathbb{R}^{3}\mbox{ can be endowed with a metric }l_{2}\notag
% \\
% &\mbox{with constant positive curvature }K=k\label{carmor2}\tag{C2}
% \end{align}
\begin{align}
&\sum_{i=1}^{m}g(x_{i})=\sum_{i=1}^{m}e^{\lambda_{0}-1+\lambda_{1}r(x_{i})}=e^{\lambda_{0}}\sum_{i=1}^{m}e^{\lambda_{1}r(x_{i})}=\notag\\
&e^{-\ln(Z(\beta))}Z(\beta)=1\label{eq:unishow}
\end{align}

Then, we show, by differentiating $\ln(Z(\beta))$ using the
substitution $x=e^{-\beta}$
\begin{align}
&\alpha=-\frac{\partial}{\partial{}\beta}\ln(Z(\beta))=-\frac{1}{\sum_{i=1}^{m}x^{r(x_{i})}}\left(\sum_{i=1}^{m}r(x_{i})x^{r(x_{i})-1}\right)(-x)=\notag\\
&\frac{\sum_{i=1}^{m}r(x_{i})x^{r(x_{i})}}{\sum_{i=1}^{m}x^{r(x_{i})}}\label{eq:alphashow}
\end{align}

And, finally,
\begin{align}
&\sum_{i=1}^{m}r(x_{i})g(x_{i})=\sum_{i=1}^{m}r(x_{i})e^{\lambda_{0}-1+\lambda_{1}r(x_{1})}=e^{\lambda_{0}-1}\sum_{i=1}^{m}r(x_{i})e^{\lambda_{1}r(x_{1})}=\notag\\
&e^{\lambda_{0}-1}\sum_{i=1}^{m}r(x_{i})x^{r(x_{i})}=\alpha{}e^{\lambda_{0}-1}\sum_{i=1}^{m}x^{r(x_{i})}=\alpha{}e^{\lambda_{0}-1}\sum_{i=1}^{m}e^{-\beta{}r(x_{i})}=\notag\\
&\alpha{}Z(\beta)e^{\lambda_{0}-1}=\alpha{}Z(\beta))e^{-\ln(Z(\beta))}=\alpha\label{eq:finalshow}
\end{align}
% \noindent\textbf{Endnotes}

% \theendnotes

% \medskip

% \noindent\textbf{References}

% \nocite{*} 
\bibliographystyle{stefan-2010-08-28}
\bibliography{bib-3306}

\end{document}
